specIR/SIRProps.v
@@ -1,5 +1,5 @@
 Require Export SIRStackproof.
-Fail Require Import RUSC AdequacyLocal.
 Require Export SIRHoareproof.
 Require Export SimSIR.
 Require Export SimSIRLocal.
+Require Import RUSC AdequacyLocal.
